Basics.v
@@ -1,0 +1,37 @@
+(* Quantifiers : Linear & Unrestricted *)
+Inductive q : Type :=
+  | qlin : q
+  | qun : q.
+
+(* Boolean Literal : True & False *)
+Inductive b : Type :=
+  | btrue : b
+  | bfalse : b.
+
+(* Names of the Variables *)
+Inductive id : Type :=
+  | Id : nat -> id.
+
+(* Type and Pretype *)
+Reserved Notation "'qty'" (at level 10).
+
+Inductive ty : Type :=
+  | ty_bool : qty
+  | ty_pair : ty -> ty -> qty
+  | ty_arrow : ty -> ty -> qty
+
+where "'qty'" := (q -> ty).
+
+Notation "T ** T'" := (ty_pair T T') (at level 20, left associativity).
+
+Notation "T --> T'" := (ty_arrow T T') (at level 40, left associativity).
+
+(* Terms *)
+Inductive tm : Type :=
+  | tmvar : id -> tm
+  | tmbool : q -> b -> tm
+  | tmif : tm -> tm -> tm -> tm
+  | tmpair : q -> tm -> tm -> tm
+  | tmsplit : tm -> id -> id -> tm -> tm
+  | tmabs : q -> id -> ty -> tm -> tm
+  | tmapp : tm -> tm -> tm.
